\documentclass{article}
\usepackage[utf8]{inputenc}
\usepackage{amsfonts}
\usepackage{amsmath}
\usepackage{ amssymb }
\usepackage[a4paper, total={6in, 10in}]{geometry} %adjusting size of pdf

\title{A9 Mini-TeX Project}
\author{Lydia Alem}
\date{November 2022}

\begin{document}

\maketitle

\section{Introduction}
%Proof question
Prove that if $n \in \mathbb{Z}^{+}$  and when sin $\not=$ 0,
$$(cos(\theta))(cos(2\theta)(cos(4\theta))(cos(8\theta)))...(cos(2^{n-1}(\theta))) = \frac{sin2^{n}(\theta)}{2^{n}sin(\theta)}$$


\section{Proof}
%base-case
Base Case: P(1) must be true: $$(cos(2^{0}(\theta))) = \frac{sin(2^{1}(\theta)}{2^{1} 
%writing the ptoley's indentity
sin(\theta)}$$ $$\fbox{\textbf{Recall the Ptoley's Indentities: $sin(\theta + \theta) = sin(2\theta) = 2(sin(\theta) cos(\theta))$ }}$$
$$cos(\theta) = \frac{2(sin(\theta)cos(\theta))}{2sin(\theta)}$$
$$cos(\theta) = cos(\theta) $$
$ \blacksquare $ %adding end of proof notation

%hypothesis:
Hypothesis: 
$$ (cos(\theta))(cos(2\theta)(cos(4\theta))(cos(8\theta)))...(cos(2^{k-1}(\theta))) = \frac{sin2^{k}(\theta)}{2^{k}sin(\theta)}$$

%proving hypothesis:
Proof(k+1) = 
$$ (cos(\theta))(cos(2\theta)(cos(4\theta))(cos(8\theta)))...(cos(2^{k-1}(\theta))cos(2^{k}(\theta)) = \frac{sin2^{k+1}(\theta)}{2^{k+1}sin(\theta)}$$

$$ =\frac{sin2^{k}(\theta)}{2^{k}sin(\theta)}(cos2^{k}(\theta))$$
%writing def of double angle

$$\fbox{\textbf{Recall the Double Angle Formula: $2sin(\alpha)cos(\alpha) = sin2(\alpha)$ }}$$



$$= \frac{sin(2\cdot2^{k}(\theta))}{2\cdot2^{k}sin(\theta)}$$

% $$\frac{sin(2^{k+1}(\theta)}{2^{k+1}}sin(\theta)$$

$$= \frac{sin(2^{k+1}(\theta)}{2^{k+1}sin(\theta)}$$
$ \blacksquare $ 


Using Proof by Induction, I was able to prove that there exists a positive number that supports the proof question. 
\end{document}
